Update sub_ptr implementation
sub_ptr is now exactly match with paper's representation

clightplus/mem/ClightPlusMem0.v
@@ -130,16 +130,26 @@ Section MODSEM.
         | _, _ => triggerUB
         end.
 
+    Definition check_val v1 v2 : itree Es unit :=
+      match v1, v2 with
+      | Vptr _ _, Vptr _ _ | Vlong _, Vlong _ => Ret tt
+      | Vptr _ _, Vlong n | Vlong n, Vptr _ _ => if Int64.eq n Int64.zero
+                                                 then triggerUB
+                                                 else Ret tt
+      | _, _ => Ret tt 
+      end.
+
     Definition sub_ptrF : Z * val * val -> itree Es val :=
       fun varg =>
         let '(sz, v1, v2) := varg in
-        mp <- trigger (PGet);;
-        m <- mp↓?;;
-        n <- (Cop._sem_ptr_sub_join_common v1 v2 m)?;;
-        if Coqlib.proj_sumbool (Coqlib.zlt 0 sz) &&
-            Coqlib.proj_sumbool (Coqlib.zle sz Ptrofs.max_signed)
-        then Ret (Vptrofs (Ptrofs.divs n (Ptrofs.repr sz)))
-        else triggerUB.
+          check_val v1 v2;;;
+          mp <- trigger (PGet);;
+          m <- mp↓?;;
+          n <- (Cop._sem_ptr_sub_join_common v1 v2 m)?;;
+          if Coqlib.proj_sumbool (Coqlib.zlt 0 sz) &&
+               Coqlib.proj_sumbool (Coqlib.zle sz Ptrofs.max_signed)
+          then Ret (Vptrofs (Ptrofs.divs n (Ptrofs.repr sz)))
+          else triggerUB.
 
     Definition non_nullF: val -> itree Es bool :=
       fun varg =>
