clightplus/compiler_proof/ClightPlusExprSim.v
@@ -167,6 +167,30 @@ Section PROOF.
         all: ii; apply n1; eapply map_blk_inj; et.
   Qed.
 
+  Lemma step_check pstate f_table modl cprog sk_mem sk tge le tle e te m tm
+    (PSTATE: pstate "Mem"%string = m↑)
+    (EQ: f_table = (ModL.add (Mem sk_mem) modl).(ModL.enclose))
+    (ME: match_e sk tge e te)
+    (MLE: match_le sk tge le tle)
+    (MGE: match_ge sk tge)
+    (MM: match_mem sk tge m tm)
+    v1 v2
+    tf tcode tcont ktr bflag r mn
+    (NEXT: paco4
+              (_sim (ModL.compile (ModL.add (Mem sk_mem) modl)) (semantics3 cprog)) r true bflag
+              (ktr (pstate, tt))
+              (State tf tcode tcont te tle tm))
+:
+    paco4
+      (_sim (ModL.compile (ModL.add (Mem sk_mem) modl)) (semantics3 cprog)) r true bflag
+      (`r0: (p_state * unit) <-
+        (EventsL.interp_Es
+          (prog f_table)
+          (transl_all mn (check_val v1 v2))
+          pstate);; ktr r0)
+      (State tf tcode tcont te tle tm).
+  Proof. unfold check_val. remove_UBcase; et. Qed.
+
   Lemma step_sub_ptr pstate f_table modl cprog sk_mem sk tge le tle e te m tm
     (PSTATE: pstate "Mem"%string = m↑)
     (EQ: f_table = (ModL.add (Mem sk_mem) modl).(ModL.enclose))
@@ -193,7 +217,9 @@ Section PROOF.
           pstate);; ktr r0)
       (State tf tcode tcont te tle tm).
   Proof.
-    unfold ccallU. sim_red. sim_tau. ss. sim_red. unfold sub_ptrF. sim_tau. repeat (sim_tau; sim_red).
+    unfold ccallU. sim_red. sim_tau. ss. sim_red. pfold_reverse.
+    unfold sub_ptrF. eapply step_check; et.
+    sim_tau. repeat (sim_tau; sim_red).
     rewrite PSTATE. sim_red. unfold unwrapU. remove_UBcase.
     repeat (sim_tau; sim_red). rewrite Any.upcast_downcast. sim_red.
     destruct Coqlib.zlt; destruct Coqlib.zle; ss.
